theories/Control/Worklist.v
@@ -1,0 +1,194 @@
+Require Import PnV.Prelude.Prelude.
+Require Import PnV.Data.FiniteSet.
+Require Import PnV.Prelude.X.
+
+Module Worklist.
+
+Section Worklist.
+
+Context {A : Type} {A_isPoset : isPoset A} {HsOrd_A : HsOrd A}.
+
+#[local] Notation "x ∈ xs" := (L.In x (FSet.data xs)).
+
+Fixpoint schedule (next : fin_ensemble A) (seen : fset A) (todo : list A) {struct next} : fset A * list A :=
+  match next with
+  | [] => (seen, todo)
+  | x :: next' => if FS.mem x seen then schedule next' seen todo else schedule next' (FS.add x seen) (x :: todo)
+  end.
+
+Theorem schedule_spec (next : fin_ensemble A) (seen : fset A) (todo : list A) seen' todo'
+  (H_OBS : schedule next seen todo = (seen', todo'))
+  : (forall x, x ∈ seen' <-> (x ∈ seen \/ L.In x next)) /\ (forall x, L.In x todo' <-> (L.In x todo \/ (L.In x next /\ ~ x ∈ seen))) /\ (length todo' + length (FSet.data seen) = length todo + length (FSet.data seen')).
+Proof.
+  revert_until next. induction next as [ | v next IH]; simpl; i.
+  - splits; intuition congruence.
+  - des_ifs.
+    + rewrite FS.mem_eq_spec in Heq.
+      find* (H_seen & H_todo & H_length) by IH.
+      splits; auto; i.
+      * rewrite H_seen. intuition congruence.
+      * rewrite H_todo. intuition congruence.
+    + rewrite FS.mem_eq_spec in Heq.
+      find* (H_seen & H_todo & H_length) by IH.
+      splits; i.
+      * rewrite H_seen, FS.in_add_eq_iff. intuition congruence.
+      * rewrite H_todo, FS.in_add_eq_iff. simpl.
+        destruct (B.decide (v = x)); intuition congruence.
+      * assert (FRESH : ~ FS.In v seen) by now rewrite FS.In_eq_iff.
+        rewrite FS.length_add in H_length by exact FRESH. cbn [length] in H_length. lia.
+Qed.
+
+Lemma schedule_no_dup (next : fin_ensemble A) (seen : fset A) (todo : list A)
+  (H_todo : forall x, L.In x todo -> x ∈ seen)
+  (NO_DUP : NoDup todo)
+  : NoDup (snd (schedule next seen todo)).
+Proof.
+  revert_until next. induction next as [ | v next IH]; simpl; i; auto; des_ifs; eapply IH; auto.
+  - intros x [EQ | IN]; rewrite FS.in_add_eq_iff; eauto.
+  - econs; auto. rewrite FS.mem_eq_spec in Heq. ii. eauto.
+Qed.
+
+Lemma schedule_seen (next : fin_ensemble A) (seen : fset A) (todo : list A) (x : A)
+  : x ∈ fst (schedule next seen todo) <-> (x ∈ seen \/ L.In x next).
+Proof.
+  destruct (schedule next seen todo) as [seen' todo'] eqn: H_OBS; simpl.
+  now obtain (? & _ & _) with H_OBS by schedule_spec.
+Qed.
+
+Lemma schedule_pending (next : fin_ensemble A) (seen : fset A) (todo : list A) (x : A)
+  : L.In x (snd (schedule next seen todo)) <-> (L.In x todo \/ (L.In x next /\ ~ x ∈ seen)).
+Proof.
+  destruct (schedule next seen todo) as [seen' todo'] eqn: H_OBS; simpl.
+  now obtain (? & ? & ?) with H_OBS by schedule_spec.
+Qed.
+
+Variable next : A -> fin_ensemble A.
+
+Variable domain : A -> Prop.
+
+Hypothesis domain_closed : forall x, domain x -> forall y, L.In y (next x) -> domain y.
+
+Hypothesis domain_finite : exists bound : nat, forall xs : fset A, forall INCL : forall x, x ∈ xs -> domain x, length (FSet.data xs) <= bound.
+
+Let state : Type :=
+  fset A * list A.
+
+Definition valid (st : state) : Prop :=
+  (forall x, x ∈ fst st -> domain x) /\ (forall x, L.In x (snd st) -> x ∈ fst st).
+
+Lemma schedule_valid (seen : fset A) (x : A) (todo : list A)
+  (VALID : valid (seen, x :: todo))
+  : valid (schedule (next x) seen todo).
+Proof.
+  destruct VALID as [DOMAIN TODO]. cbn in DOMAIN, TODO.
+  destruct (schedule (next x) seen todo) as [seen' todo'] eqn: H_OBS; simpl.
+  obtain (SEEN & PENDING & LENGTH) with H_OBS by schedule_spec.
+  split; cbn; i.
+  - rewrite SEEN in H. destruct H; eauto.
+  - rewrite PENDING in H. rewrite SEEN. intuition eauto.
+Qed.
+
+Inductive transition : state -> state -> Prop :=
+  | transition_step (seen : fset A) (x : A) (todo : list A)
+    (VALID : valid (seen, x :: todo))
+    : transition (seen, x :: todo) (schedule (next x) seen todo).
+
+Definition measure (bound : nat) (st : state) : nat :=
+  bound - length (FSet.data (fst st)) + length (snd st).
+
+Lemma transition_decreases (bound : nat) (st : state) (st' : state)
+  (BOUND : forall xs : fset A, forall INCL : forall x, x ∈ xs -> domain x, length (FSet.data xs) <= bound)
+  (STEP : transition st st')
+  : measure bound st' < measure bound st.
+Proof.
+  inv STEP.
+  destruct (schedule (next x) seen todo) as [seen' todo'] eqn: H_OBS; simpl.
+  obtain (SEEN & PENDING & LENGTH) with H_OBS by schedule_spec.
+  obtain [DOMAIN' TODO'] with VALID by schedule_valid.
+  destruct VALID as [DOMAIN TODO]. cbn in DOMAIN, DOMAIN'.
+  obtain OLD with DOMAIN by BOUND.
+  obtain NEW with DOMAIN' by BOUND.
+  rewrite H_OBS in NEW. unfold measure. simpl in *. lia.
+Qed.
+
+Lemma transition_hasSN
+  : SN.hasSN transition.
+Proof.
+  destruct domain_finite as [bound BOUND]. intros st; pattern st; revert st.
+  eapply well_founded_induction with (R := fun st => fun st' => measure bound st < measure bound st').
+  - exact (well_founded_ltof state (measure bound)).
+  - intros st IH. econs. i. eapply IH.
+    eapply transition_decreases; eauto.
+Qed.
+
+Fixpoint run (st : state) (VALID : valid st) (NORMAL : SN.sn transition st) {struct NORMAL} : fset A.
+Proof.
+  destruct st as [seen [ | x todo]].
+  - exact seen.
+  - exact (run (schedule (next x) seen todo) (schedule_valid seen x todo VALID) (SN.sn_inv (seen, x :: todo) NORMAL (schedule (next x) seen todo) (transition_step seen x todo VALID))).
+Defined.
+
+Fixpoint run_sound (P : A -> Prop) (st : state)
+  (CLOSED : forall x, P x -> forall y, L.In y (next x) -> P y)
+  (sn_st : SN.sn transition st)
+  (H_valid : valid st)
+  (INITIAL : forall x, x ∈ fst st -> P x)
+  : forall x, x ∈ run st H_valid sn_st -> P x.
+Proof.
+  destruct sn_st as [sn_st_inv]. destruct st as [seen [ | x todo]]; simpl.
+  - exact INITIAL.
+  - set (st' := schedule (next x) seen todo).
+    assert (PRESERVED : forall y, y ∈ fst st' -> P y).
+    { subst st'. intros y H_y. rewrite schedule_seen in H_y. destruct H_y; eauto.
+      eapply CLOSED; eauto. eapply INITIAL. eapply H_valid. cbn; auto.
+    }
+    exact (run_sound P st' CLOSED (sn_st_inv st' (transition_step seen x todo H_valid)) (schedule_valid seen x todo H_valid) PRESERVED).
+Qed.
+
+Fixpoint run_complete (st : state)
+  (sn_st : SN.sn transition st)
+  (VALID : valid st)
+  (CLOSED : forall x, x ∈ fst st -> forall y, L.In y (next x) -> (y ∈ fst st \/ L.In x (snd st)))
+  : (forall x, x ∈ fst st -> x ∈ run st VALID sn_st) /\ (forall x, forall y, x ∈ run st VALID sn_st -> L.In y (next x) -> y ∈ run st VALID sn_st).
+Proof.
+  destruct sn_st as [sn_st_inv]. destruct st as [seen [ | v todo]]; cbn [run].
+  - split; i; auto. find* [IN | []] by CLOSED. exact IN.
+  - enough (NEXT_CLOSED : forall x, x ∈ fst (schedule (next v) seen todo) -> forall y, L.In y (next x) -> (y ∈ fst (schedule (next v) seen todo) \/ L.In x (snd (schedule (next v) seen todo)))).
+    { obtain [MONOTONE CLOSED_out] with (sn_st_inv _ (transition_step seen v todo VALID)) (schedule_valid seen v todo VALID) NEXT_CLOSED by run_complete.
+      split; auto. i. eapply MONOTONE. rewrite schedule_seen. auto.
+    }
+    intros x IN y EDGE. rewrite schedule_seen in IN. simpl in *. destruct IN as [IN | IN].
+    + find* [IN' | [EQ | IN_todo]] by CLOSED.
+      * left. rewrite schedule_seen. auto.
+      * subst x. left. rewrite schedule_seen. auto.
+      * right. rewrite schedule_pending. auto.
+    + destruct (FS.mem x seen) eqn: OBS.
+      * rewrite FS.mem_eq_spec in OBS. find* [IN_y | [EQ | IN_todo]] by CLOSED.
+        { left. rewrite schedule_seen. auto. }
+        { subst x. left. rewrite schedule_seen. auto. }
+        { right. rewrite schedule_pending. auto. }
+      * rewrite FS.mem_eq_spec in OBS. right. rewrite schedule_pending. auto.
+Qed.
+
+Definition closure (initial : fset A) (H_initial : forall x : A, forall IN : x ∈ initial, domain x) : fset A :=
+  run (initial, FSet.data initial) (conj H_initial (fun x : A => fun IN : x ∈ initial => IN)) (SN.sn_intro_generator 64 transition_hasSN (initial, FSet.data initial)).
+
+Corollary closure_sound (P : A -> Prop) (initial : fset A)
+  (H_initial : forall x, x ∈ initial -> domain x)
+  (CLOSED_P : forall x, forall y, P x -> L.In y (next x) -> P y)
+  (INITIAL_P : forall x, x ∈ initial -> P x)
+  : forall x, x ∈ closure initial H_initial -> P x.
+Proof.
+  eapply run_sound; i; eauto.
+Qed.
+
+Corollary closure_complete (initial : fset A)
+  (H_initial : forall x, x ∈ initial -> domain x)
+  : (forall x, x ∈ initial -> x ∈ closure initial H_initial) /\ (forall x, forall y, x ∈ closure initial H_initial -> L.In y (next x) -> y ∈ closure initial H_initial).
+Proof.
+  eapply run_complete with (st := (initial, FSet.data initial)); cbn; i; auto.
+Qed.
+
+End Worklist.
+
+End Worklist.
